
#### 2.1 Ambiguity

Ambiguity arises when a grammar allows multiple parse trees for a single input string. 

**Example:**
![[Pasted image 20241211175908.png]]
Consider the grammar G:  `E → E+E / E*E / (E) / idf / cstent`

To resolve ambiguity, we introduce operator precedence and associativity rules. Assuming standard arithmetic precedence ( '*'  and '/' have higher precedence than '+' and '-' , and operators are left-associative), we obtain the unambiguous grammar G':

- `E → E + T / T`
- `T → T * F / F`
- `F → (E) / idf / cstent`


Okay, here's a note on how to remove ambiguity according to the audio and the provided image:

**Removing Ambiguity in Grammar**

Based on the audio and the image, ambiguity in grammar can be removed by creating levels of precedence and using parsing. Here's a breakdown:

**1. Create Levels of Non-Terminals (Precedence):**

*   **Identify Ambiguous Grammar:** The image shows an example of an ambiguous grammar rule: `E -> E + E | E * E | id`. This rule can lead to different interpretations of the same expression (e.g., `id + id * id`).
*   **Establish Precedence:** To resolve this, the speaker suggests creating levels of precedence. In the image, these are represented as:
    *   `E` - First Level of precedence.
    *   `T` - Second Level of precedence.
    *   `F` - Generating basic units (terminals) in the expression.

**2. Rewrite Grammar with Additional Rules:**

*   Based on the precedence levels, the ambiguous grammar rule is rewritten using new non-terminals (`T` and `F`) to enforce the desired order of operations:

    ```
    E -> E + T | T
    T -> T * F | F
    F -> id
    ```

*   **Example:**
    For string `id + id * id`

**3. Parsing:**

*   **Construct a Parse Tree:** A parse tree is created to visually represent the structure of the expression according to the new grammar rules. The image shows an example of a parse tree for the expression `id + id * id`.
*   **Analyze the Parse Tree:** By examining the parse tree, we can determine the correct order of operations based on the hierarchy of non-terminals (`E`, `T`, and `F`).

**4. Applying the Correct Parsing (Healthy Parsing):**

*   The audio emphasizes the importance of using the "correct parsing" or "healthy parsing." This means constructing the parse tree in a way that accurately reflects the intended precedence levels.
*   By following the correct parsing, we can ensure that the expression is evaluated according to the defined order of operations (e.g., multiplication before addition).

**In summary:**

The audio and image illustrate that ambiguity in grammar can be removed by:

1. Defining levels of precedence for operators.
2. Rewriting the grammar rules to incorporate these precedence levels using new non-terminals.
3. Using parsing to create a parse tree that visually represents the expression's structure.
4. Applying the correct parsing to ensure the expression is evaluated according to the intended order of operations.

This process ensures a clear and unambiguous interpretation of grammatical expressions.


[[3.6 Dangling If Else]]

---


#### 2.2 Left Recursion

### Example 1: **Single Rule Direct Left Recursion**

#### Problem

Grammar:

```plaintext
A → Aα | β
```

This rule is left-recursive because `A` appears on the left-hand side at the beginning of its production.

#### Solution

Eliminate left recursion by rewriting:

1. Introduce a new non-terminal, `A'`.
2. Rewrite:
    - A→βA′A → βA'
    - A′→αA′∣εA' → αA' | ε

#### Result

```plaintext
A → βA'
A' → αA' | ε
```

---

### Example 2: **Multiple Direct Left Recursive Rules**

#### Problem

Grammar:

```plaintext
A → Aα | Aβ | γ
```

#### Solution

1. Rewrite:
    - A→γA′
    - A′→αA′∣βA′∣ε

#### Result

```plaintext
A → γA'
A' → αA' | βA' | ε
```

---

### Example 3: **Indirect Left Recursion**

#### Problem

Grammar:

```plaintext
A → Bα
B → Aβ | γ
```

#### Solution

Indirect left recursion involves substitutions to make it direct. Substitute `B` in `A`:

1. A→(Aβ∣γ)αA → (Aβ | γ)α
2. Rewrite with direct left recursion eliminated:
    - A→γαA′A → γαA'
    - A′→βαA′∣εA' → βαA' | ε

#### Result

```plaintext
A → γαA'
A' → βαA' | ε
B → Aβ | γ
```

---

### Example 4: **Complex Indirect Left Recursion**

#### Problem

Grammar:

```plaintext
A → Bα | δ
B → Cβ | ε
C → Aγ | ζ
```

#### Solution

Resolve dependencies and substitute to make recursion explicit:

1. Substitute `C` into `B`, and then `B` into `A`.
2. Rewrite `A`:
    - A→δA′A → δA'
    - A′→αA′∣γA′∣εA' → αA' | γA' | ε

#### Result

```plaintext
A → δA'
A' → αA' | γA' | ε
B → ζβ | ε
C → δγ | ζ
```

---

### Example 5: **Grammar with Mixed Recursive and Non-Recursive Rules**

#### Problem

Grammar:

```plaintext
A → Aa | Ab | c | d
```

#### Solution

1. Factor out common prefixes and eliminate direct left recursion:
    - A→cA′∣dA′A → cA' | dA'
    - A′→aA′∣bA′∣εA' → aA' | bA' | ε

#### Result

```plaintext
A → cA' | dA'
A' → aA' | bA' | ε
```

---

### General Tip for Elimination

1. **Identify left recursion** (direct or indirect).
2. **Substitute indirect recursion** to make it direct.
3. **Rewrite grammar rules** by introducing new non-terminals to factor recursive productions and terminate recursion.

#### 2.3 Left Factoring

Left factoring eliminates common prefixes in production rules to avoid backtracking during parsing.

A grammar is unfactored if a production rule has the form: `A → αA1 / αA2 / ... / αAn / β1 / β2 / ... / βm`

**Factoring:**

Rewrite the rule as:

- `A → αA' / β1 / β2 / ... / βm`
- `A' → A1 / A2 / ... / An`

Repeat for all production rules with common prefixes.

**Example:**

```
A → abC / aAB / caF 
```
After left factoring:
```
A → aA' / caF
A’ → bC / AB
```
